execution_invariants_s.thy
@@ -11,7 +11,7 @@ text {* This theory includes proof for invariants that hold for all single-invoc
 
 
 
-definition initialStates :: "('localState, 'any) prog \<Rightarrow> invocation \<Rightarrow> ('localState, 'any) state set"  where
+definition initialStates :: "('localState, 'any::valueType) prog \<Rightarrow> invocation \<Rightarrow> ('localState, 'any) state set"  where
   "initialStates progr i \<equiv> {
     (S\<lparr>localState := (localState S)(i \<mapsto> initState),
        currentProc := (currentProc S)(i \<mapsto> impl),
